[K-th Symbol in Grammar](https://leetcode.com/problems/k-th-symbol-in-grammar/)
length
n=1 0 2^(1-1) = 1
n=2 01 2^(2-1) = 2
n=3 0110 2^(3-1) = 4
n=4 01101001 2^(4-1) = 8
n=5 0110100110010110 2^(5-1) = 16

-   observe that **first half of elements in nth row = total elements in (n-1)th row**

```cpp
class Solution {
public:
    int kthGrammar(int n, int k) {
        if(n == 1 && k == 1) return 0;
        int mid = pow(2, n-1)/2;//length is 2^(n-1)
        if(k <= mid){
            return kthGrammar(n-1, k);
        }
        else return !kthGrammar(n-1, k-mid);
    }
};
```
